begin modeling repair attempt 2

papers/116_stefan_rass/LD_Issues.thy
@@ -2,11 +2,95 @@ theory LD_Issues
   imports L0
 begin
 
+
+\<comment> \<open>Decode a pair of words \<open>(l, x) \<in> {0,1}* \<times> {0,1}*\<close> from its encoded form "\<open>l\<parallel>x \<in> {0,1}*\<close>".
+
+  The encoding defined by this should have \<open>l\<close> encoded in the upper (more significant) bits of \<open>l\<parallel>x\<close>.
+
+  This is undefined for now, as the restricted alphabet does not allow the obvious method
+  of using a separation symbol that can not occur in \<open>l\<close>.
+  (It suffices to restrict this condition to \<open>l\<close>, since after encountering the symbol
+  the "rest" of \<open>w\<close> is determined \<open>x\<close>.)
+
+  A possible solution for this would be to use another encoding for \<open>l\<close>,
+  such as \<^const>\<open>decode_word\<close>, defined in \<^theory>\<open>OWF.Complexity\<close>.
+  However, this method may have unintended side-effects, as the encoding increases the length,
+  which is critical in proving some of the further lemmas.\<close>
+
+\<comment> \<open>what if \<open>l = 1\<^sup>n\<close> and \<open>\<cent> = 0\<close>? then \<open>w = 1\<^sup>l0w\<close>\<close>
+
+definition decode_pair :: "word \<Rightarrow> word \<times> word"
+  where "decode_pair \<equiv> undefined"
+
+
+context tht_assms
+begin
+
+\<comment> \<open>Alternative \<open>L\<^sub>D\<close>.
+
+  Note: this is not intended to replace \<^const>\<open>L\<^sub>D\<close>.
+  The further proof uses the similarity of \<open>L\<^sub>D\<close> and \<open>L\<^sub>D''\<close>
+  to prove properties of \<open>L\<^sub>D''\<close> via reduction to \<open>L\<^sub>D\<close>.
+
+  Construction: Given a word \<open>w\<close>.
+  Split the word \<open>w\<close> into \<open>(l, x)\<close> using \<^const>\<open>decode_pair\<close>.
+  Define \<open>v\<close> as the \<open>log\<^sub>2(l)\<close> most-significant-bits of \<open>x\<close>.
+  Remove the arbitrary-length \<open>1\<^sup>+0\<close>-prefix from \<open>v\<close> to retain the pure encoding of \<open>M\<^sub>v\<close>.
+  If \<open>M\<^sub>v\<close> rejects \<open>v\<close> within \<open>T(len(x))\<close> steps, \<open>w \<in> L\<^sub>D''\<close> holds.
+
+  Note that in this version, using \<^const>\<open>time_bounded_word\<close> is not possible,
+  as the word that determines the time bound (\<open>x\<close>) differs from the input word (\<open>v\<close>).
+  The alternative version shown in @{thm time_bounded_altdef} is used for simplicity.\<close>
+
+definition (in tht_assms) L\<^sub>D'' :: lang
+  where "L\<^sub>D'' \<equiv> {w. 
+      let (l, x) = decode_pair w;
+          v = drop (length x - clog (l)\<^sub>2) x;
+          M\<^sub>v = decode_TM (strip_al_prefix v) in
+      rejects M\<^sub>v v \<and> is_final (steps0 (1, <v>\<^sub>t\<^sub>p) M\<^sub>v (tcomp\<^sub>w T x))
+    }"
+
+end \<comment> \<open>\<^locale>\<open>tht_assms\<close>\<close>
+
+
+context tht_sq_assms
+begin
+
 lemma
+  fixes w
+  defines "w' \<equiv> adj_sq\<^sub>w w"
+  defines "l \<equiv> fst (decode_pair w)"
+    and "x \<equiv> snd (decode_pair w)"
+    and "l' \<equiv> fst (decode_pair w')"
+    and "x' \<equiv> snd (decode_pair w')"
+  defines "v \<equiv> drop (length x - clog (l)\<^sub>2) x"
+    and "v' \<equiv> drop (length x' - clog (l')\<^sub>2) x'"
+    (* need some assumption that fixes the length of l in a way that allows this to work *)
+  shows "v' = v"
+proof -
+  oops
+
+
+lemma L\<^sub>D_adj_sq_iff:
+  fixes w
+  defines l: "l \<equiv> fst (decode_pair w)"
+    and w': "w' \<equiv> adj_sq\<^sub>w w"
+  assumes "length w \<ge> 20"
+    and "clog (l)\<^sub>2 \<le> clog (length w)" (* new *)
+  shows "w' \<in> L\<^sub>D'' \<longleftrightarrow> w \<in> L\<^sub>D''"
+proof -
+  from \<open>length w \<ge> 20\<close> have "shared_MSBs (clog (length w)) w w'" unfolding w' by (rule adj_sq_sh_pfx_log)
+  then have "length w' = length w" by (elim sh_msbE[symmetric])
+  oops
+
+end \<comment> \<open>\<^locale>\<open>tht_sq_assms\<close>\<close>
+
+
+lemma (* relation between two similar, but not equivalent propositions *)
   assumes "tm_wf0 M_w"
     and "M_w \<noteq> Rejecting_TM"
   shows "TM_decode_pad w = M_w \<longleftrightarrow> strip_al_prefix (strip_exp_pad w) = encode_TM M_w"
-proof (intro iffI)
+proof (rule iffI)
   assume *: "TM_decode_pad w = M_w"
   with assms(2) have h1: "is_encoded_TM (strip_al_prefix (strip_exp_pad w))"
     unfolding TM_decode_pad_def decode_TM_def by argo
@@ -28,127 +112,5 @@ next
   show "TM_decode_pad w = M_w" unfolding TM_decode_pad_def *
     by (rule codec_TM) fact
 qed
-
-
-context tht_assms
-begin
-
-text\<open>Alternative formulation, intended to fix the issues of \<^const>\<open>L\<^sub>D\<close> for Lemma 4.6
-  and \<^const>\<open>L\<^sub>D'\<close> for the THT.\<close>
-
-definition L\<^sub>D'' :: lang
-  where LD''_def: "L\<^sub>D'' \<equiv> {w. \<exists>M\<^sub>w. w = encode_TM M\<^sub>w \<and> rejects M\<^sub>w w \<and> time_bounded_word T M\<^sub>w w}"
-
-definition L\<^sub>D''' :: lang
-  where LD'''_def: "L\<^sub>D''' \<equiv> {w. let M\<^sub>w = TM_decode_pad w in
-                  (\<exists>M\<^sub>w. w = encode_TM M\<^sub>w) \<and> rejects M\<^sub>w w \<and> time_bounded_word T M\<^sub>w w}"
-
-
-theorem time_hierarchy': "L\<^sub>D' \<in> DTIME(T) - DTIME(t)"
-proof
-  show "L\<^sub>D' \<in> DTIME(T)" sorry (* unchanged *)
-
-  have "L \<noteq> L\<^sub>D'" if "L \<in> DTIME(t)" for L
-  proof -
-    from \<open>L \<in> DTIME(t)\<close> obtain M\<^sub>w where "decides M\<^sub>w L" and "time_bounded t M\<^sub>w" and "tm_wf0 M\<^sub>w" ..
-
-    let ?n = "length (encode_TM M\<^sub>w) + 2"
-    obtain l where "T(2*l) \<ge> t(2*l)" and "clog l \<ge> ?n" sorry (* unchanged *)
-    obtain w where "length w = l" and dec_w: "TM_decode_pad w = M\<^sub>w"
-      using \<open>tm_wf0 M\<^sub>w\<close> \<open>clog l \<ge> ?n\<close> by (rule embed_TM_in_len)
-
-    let ?w = "strip_al_prefix (strip_exp_pad w)"
-    have "?w \<in> L \<longleftrightarrow> w \<notin> L\<^sub>D'"
-    proof
-      assume "?w \<in> L"
-      moreover from \<open>decides M\<^sub>w L\<close> have "?w \<notin> L \<longleftrightarrow> rejects M\<^sub>w ?w" unfolding decides_def by blast
-      ultimately have "\<not> rejects M\<^sub>w ?w" by blast
-      then show "w \<notin> L\<^sub>D'" unfolding LD'_def mem_Collect_eq dec_w Let_def by presburger
-    next
-      assume "w \<notin> L\<^sub>D'"
-      moreover have "time_bounded_word T M\<^sub>w ?w" sorry (* probably works *)
-      ultimately have "\<not> rejects M\<^sub>w ?w" unfolding LD'_def dec_w mem_Collect_eq Let_def by blast
-      with \<open>decides M\<^sub>w L\<close> show "?w \<in> L" unfolding decides_def by blast
-    qed
-
-    have "w \<in> L \<longleftrightarrow> w \<notin> L\<^sub>D'"
-    proof
-      assume "w \<in> L"
-      moreover from \<open>decides M\<^sub>w L\<close> have "w \<notin> L \<longleftrightarrow> rejects M\<^sub>w w" unfolding decides_def by blast
-      ultimately have "\<not> rejects M\<^sub>w w" by blast
-      then show "w \<notin> L\<^sub>D'" unfolding LD'_def mem_Collect_eq dec_w Let_def by presburger (* nope *)
-    next
-      assume "w \<notin> L\<^sub>D'"
-      moreover have "time_bounded_word T M\<^sub>w w"
-      proof (rule time_bounded_word_mono)
-        from \<open>T(2*l) \<ge> t(2*l)\<close> show "real (T (tape_size <w>\<^sub>t\<^sub>p)) \<ge> real (t (tape_size <w>\<^sub>t\<^sub>p))"
-          unfolding tape_size_input \<open>length w = l\<close> by (rule of_nat_mono)
-        from \<open>time_bounded t M\<^sub>w\<close> show "time_bounded_word t M\<^sub>w w" ..
-      qed
-      ultimately have "\<not> rejects M\<^sub>w w" unfolding LD'_def dec_w mem_Collect_eq Let_def by blast (* nope *)
-      with \<open>decides M\<^sub>w L\<close> show "w \<in> L" unfolding decides_def by blast
-    qed
-    then show "L \<noteq> L\<^sub>D'" by blast
-  qed
-  then show "L\<^sub>D' \<notin> DTIME(t)" by blast
-qed
-
-theorem time_hierarchy'': "L\<^sub>D'' \<in> DTIME(T) - DTIME(t)"
-proof
-  show "L\<^sub>D'' \<in> DTIME(T)" sorry (* unchanged *)
-
-  have "L \<noteq> L\<^sub>D''" if "L \<in> DTIME(t)" for L
-  proof -
-    from \<open>L \<in> DTIME(t)\<close> obtain M\<^sub>w where "decides M\<^sub>w L" and "time_bounded t M\<^sub>w" and "tm_wf0 M\<^sub>w" ..
-
-    let ?n = "length (encode_TM M\<^sub>w) + 2"
-    obtain l where "T(2*l) \<ge> t(2*l)" and "clog l \<ge> ?n" sorry (* unchanged *)
-    obtain w where "length w = l" and dec_w: "TM_decode_pad w = M\<^sub>w"
-      using \<open>tm_wf0 M\<^sub>w\<close> \<open>clog l \<ge> ?n\<close> by (rule embed_TM_in_len)
-
-    have "w \<in> L \<longleftrightarrow> w \<notin> L\<^sub>D''"
-    proof
-      assume "w \<in> L"
-      moreover from \<open>decides M\<^sub>w L\<close> have "w \<notin> L \<longleftrightarrow> rejects M\<^sub>w w" unfolding decides_def by blast
-      ultimately have "\<not> rejects M\<^sub>w w" by blast
-      then show "w \<notin> L\<^sub>D''" unfolding LD''_def mem_Collect_eq dec_w Let_def by presburger (* nope *)
-    next
-      assume "w \<notin> L\<^sub>D''"
-      moreover have "time_bounded_word T M\<^sub>w w"
-      proof (rule time_bounded_word_mono)
-        from \<open>T(2*l) \<ge> t(2*l)\<close> show "real (T (tape_size <w>\<^sub>t\<^sub>p)) \<ge> real (t (tape_size <w>\<^sub>t\<^sub>p))"
-          unfolding tape_size_input \<open>length w = l\<close> by (rule of_nat_mono)
-        from \<open>time_bounded t M\<^sub>w\<close> show "time_bounded_word t M\<^sub>w w" ..
-      qed
-      ultimately have "\<not> rejects M\<^sub>w w" unfolding LD''_def dec_w mem_Collect_eq Let_def by blast (* nope *)
-      with \<open>decides M\<^sub>w L\<close> show "w \<in> L" unfolding decides_def by blast
-    qed
-    then show "L \<noteq> L\<^sub>D''" by blast
-  qed
-  then show "L\<^sub>D'' \<notin> DTIME(t)" by blast
-qed
-
-end (* context tht_assms *)
-
-
-context tht_sq_assms
-begin
-
-lemma L\<^sub>D_adj_sq_iff:
-  fixes w
-  assumes l: "length w \<ge> 20"
-  defines w': "w' \<equiv> adj_sq\<^sub>w w"
-  shows "w' \<in> L\<^sub>D'' \<longleftrightarrow> w \<in> L\<^sub>D''"
-proof -
-  from \<open>length w \<ge> 20\<close> have "shared_MSBs (clog (length w)) w w'" unfolding w' by (rule adj_sq_sh_pfx_log)
-  then have "length w' = length w" by (elim sh_msbE[symmetric])
-  then have len: "tape_size <w'>\<^sub>t\<^sub>p = tape_size <w>\<^sub>t\<^sub>p" unfolding tape_size_input by (rule arg_cong)
-  from l have dec: "TM_decode_pad w' = TM_decode_pad w" unfolding w' by (rule adj_sq_TM_dec)
-  from l have pad: "strip_exp_pad w' = strip_exp_pad w" unfolding w' by (rule adj_sq_exp_pad)
-  show "w' \<in> L\<^sub>D'' \<longleftrightarrow> w \<in> L\<^sub>D''" unfolding LD''_def mem_Collect_eq unfolding dec pad len
-  oops
-
-end (* context tht_sq_assms *)
-
 
 end
